\documentclass[12pt]{article}
\usepackage{amssymb}
\usepackage{amsmath}
\usepackage{tikz}

\newtheorem{theorem}{Theorem}


\begin{document}

\title{Trying to converge to an equilibrium flow}
\maketitle

Throughout, Vickrey queuing model is used.

\section*{Iterative Model}

TBD

$$ h_P^{(i+1)}(\theta) = \left(1 - \alpha( d_P^{(i)}(\theta)) \right) \cdot h_P^{i}(\theta) + \frac{ \mathbb{I}_{ \{d_P^{(i)} < \varepsilon \}} (\theta) }{\sum_{P'} \mathbb{I}_{ \{d_{P'}^{(i)} < \varepsilon \}} (\theta)} \cdot \left( \sum_{P'} \alpha( d_P^{(i)}(\theta)) \cdot h_P^{i}(\theta) \right).$$

%\sum_{} \mathbb{I}_{d_P^{i}(\theta) < \varepsilon}

\section*{Dynamic Replicator Model}

Let $\mathcal{P}$ be a collection of $s$-$t$ paths. At time $\theta$, each path $P$ receives a fraction $h_P(\theta)$ of the total inflow $u(\theta)$. We are considering the replication dynamic: 

$$ \dot{h}_P = R \cdot h_P \cdot a_P, \quad ~\forall P \in \mathcal{P}, $$
where $R > 0$ is a constant, $a_P = \phi_P - \sum_{P' \in \mathcal{P}} h_{P'} \cdot \phi_{P'}$ is advantage function based on fitness $\phi$. 

 Role of the fitness can be played by negative signed average experienced travel time of the particles:
%($\theta_l = \max( \theta - w, 0 )$)
$$ \phi^{a.t.}_P(\theta, h) = - \frac{1} {F_P^+(\theta)} \left( \int_{0}^{\theta} F_P^+(\psi) d \psi - \int_{0}^{\theta} F_P^{-} (\psi) d \psi \right) .$$
Above, $F_P^+(\cdot)$, $F_P^-(\cdot)$ denote functions of accumulated path in- and outflow.

Another option is  negative signed last available travel time:
$$ \phi^{l.t.}_P(\theta, h) = -1 \cdot \begin{cases} \theta, & 0 \leq \theta < T_P(0) \\ \theta - T_P^{-1}(\theta), & \theta \geq T_P(0) \end{cases} ,$$
 $T_P(\cdot)$ is path exit time function.
 
Finally, utilising constant predictors for queues, one can predict path exit times $ \hat{T}_P $ and use negative predicted travel time:
$$ \phi^{p.t.}_P(\theta, h) = - (\hat{T}_P(\theta) - \theta) .$$
If path $P$ has only one edge, then $ \hat{T}_P(\cdot) \equiv T_P(\cdot) $.

\subsection*{Considered Instance}

Consider simple network with two parallel edges on Figure \ref{fig:instance}. Let upper edge have index $0$ and lower $1$. We consider inflow $u(\theta) \equiv U$.

\begin{figure}
	\begin{center}
		\begin{tikzpicture}[scale=0.2]
			\tikzstyle{every node}+=[inner sep=0pt]
			\draw [black] (7.2,-8.7) circle (3);
			\draw (7.2,-8.7) node {$s$};
			\draw [black] (27.1,-8.7) circle (3);
			\draw (27.1,-8.7) node {$t$};
			\draw [black] (9.808,-7.224) arc (114.62656:65.37344:17.62);
			\fill [black] (24.49,-7.22) -- (23.97,-6.44) -- (23.56,-7.35);
			\draw (17.15,-5.12) node [above] {$\tau=1, \nu=2$};
			\draw [black] (24.706,-10.5) arc (-58.92949:-121.07051:14.642);
			\fill [black] (24.71,-10.5) -- (23.76,-10.48) -- (24.28,-11.34);
			\draw (17.15,-13.1) node [below] {$\tau=2, \nu=3$};
		\end{tikzpicture}
	\end{center}
	\caption{Simple network}
	\label{fig:instance}
\end{figure}

The equilibrium flow is achieved as follows: all the inflow is redirected to the shorter edge, until both edges achieve equal costs, then the distribution is proportional to the capacities.
$$ h^*_0(\theta) = \begin{cases} 1, & 0 \leq \theta < (\tau_1 - \tau_0) \frac{\nu_0}{U - \nu_0} \\  \frac{\nu_0}{U}, &\theta \geq (\tau_1 - \tau_0) \frac{\nu_0}{U - \nu_0} \end{cases}, \quad h^*_1(\theta) = 1 - h^*_0(\theta) .$$


\subsection*{Numerical Approximation}

 show numerically computed inflow shares and fitness of replicator flow with initial condition $h_0(0) = h_1(0) = \frac{1}{2}$. The following approximation was used:

$$ h_P(\theta + \Delta\theta) \approx \frac{ h_P(\theta) \cdot e^{ R \cdot a_P \cdot \Delta \theta }} { \sum_{P'}  h_{P'}(\theta) \cdot e^{ R \cdot a_{P'} \cdot \Delta\theta } } .$$

By construction of the initial dynamic $\sum_{P'}  h_{P'}(\theta) \cdot e^{ R \cdot a_{P'} \cdot \Delta\theta } = 1 + o(\Delta \theta)$. Normalisation is required to remain on simplex.

\newpage

\subsection*{Stabilizing Dynamics (max demand)}

\subsubsection*{Logit Regularization}

One can use modify the fitness using logit regularizer:
$$ \phi^{\text{reg}}_P(\theta, h) = \phi_P(\theta, h) - \lambda e^{-\gamma \cdot \theta} \ln{ h_P(\theta) }, $$
where $\lambda > 0$ is a scaling constant, $\gamma > 0$ is regularization decay. Figure \ref{fig:reg_pred_tt} shows amplitude drops for different 

\begin{figure}
	\includegraphics[width=0.9\textwidth]{img/reg_pred_tt.eps}
	\caption{Predicted travel time with logit regularization $\lambda=1$}
	\label{fig:reg_pred_tt}

\end{figure}

\subsubsection*{Projected Travel Times}

If we use projected queue values $\hat{q}^{\delta}_e(\theta') = q_e(\theta) + \frac{q_e(\theta) - q_e(\theta - \delta)}{\delta} \cdot (\theta' - \theta)$ to estimate upcoming travel times, we can use fitness $$ \phi^{\text{proj t.t.}}(\theta, h) = -(t_P(\theta) + w \cdot \frac{\partial t_P}{\partial \theta}(\theta)) \approx - ( \tau_P + \frac{1}{\nu_P} \hat{q}^{\delta}_e(\theta + w) ). $$  Projection window $w$ is a paramater. 

\subsubsection*{Analysis}
Denote  $\Phi(\theta) := t_0(\theta) - t_1(\theta)$,  $\mathbb{I}_{q_e}(\theta) := \begin{cases} 1, q_e(\theta) > 0 \text{ or } f_e^+(\theta) \geq \nu_e \\ 0, \text{ otherwise}\end{cases}$.
\\
Queue $q_e$ "activates" at the moment $ \theta_{q_e} $ s.t. $f_e^+( \theta_{q_e}) = \nu_e $ and deactivates at the moment $\theta'_{q_e}$ s.t. $\int_{\theta_{q_e}}^{ \theta'_{q_e}} (f_e^+(z) - \nu_e)  dz  = 0$.
\\
We can write the derivative of $\Phi$ as

 $$ \quad \dot{\Phi} = \left(\frac{U h_0}{\nu_0} - 1 \right) \mathbb{I}_{q_0} - \left(\frac{U (1 - h_0)}{\nu_1} - 1 \right)\mathbb{I}_{q_1} $$
and substitute in replication DE with projected travel times as fitnesses:
 $$ \dot{h_0} = Rh(\phi_0 - h_0\phi_0 -(1-h_0)\phi_1) = Rh_0(1-h_0)(\phi_0 - \phi_1) = -Rh_0(1-h_0)(\Phi + w \dot{\Phi} ) $$
There are 4 different cases:
 \begin{enumerate}
 
	\item $  \mathbb{I}_{q_0} = 1,  \mathbb{I}_{q_1} = 1 $
		
	$$ h_0 = \frac{\dot{\Phi} + \frac{U}{\nu_1}}{\frac{U}{\nu_0} + \frac{U}{\nu_1}} \stackrel{\dot \Phi \to 0}{\to} \frac{\nu_0}{\nu_0 + \nu_1 },\quad 1 - h_0 = \frac{\frac{U}{\nu_0} - \dot{\Phi}}{{\frac{U}{\nu_0} + \frac{U}{\nu_1}}} . $$

$$ \frac{\ddot{\Phi}}{\frac{U}{\nu_0} + \frac{U}{\nu_1}} = -R \frac{\dot{\Phi} + \frac{U}{\nu_1}}{\frac{U}{\nu_0} + \frac{U}{\nu_1}} \cdot \frac{\frac{U}{\nu_0} - \dot{\Phi}}{\frac{U}{\nu_0} + \frac{U}{\nu_1}} \cdot (\Phi + w \dot{\Phi}) $$

$$ \ddot{\Phi} \approx - k (\Phi + w \dot{\Phi}), \quad k = R \frac{U}{\nu_0 + \nu_1} $$

 
	
	\item  $  \mathbb{I}_{q_0} = 1,  \mathbb{I}_{q_1} = 0 $
	
		$$ h_0 = \frac{\dot{\Phi} + 1}{\frac{U}{\nu_0}} \stackrel{\dot \Phi \to 0}{\to} \frac{\nu_0}{U},\quad 1 - h_0 = \frac{\frac{U}{\nu_0} - 1 - \dot{\Phi}}{{\frac{U}{\nu_0} }} . $$

$$ \frac{\ddot{\Phi}}{\frac{U}{\nu_0} } = -R \frac{\dot{\Phi} + 1}{\frac{U}{\nu_0} } \cdot \frac{\frac{U}{\nu_0} - 1 - \dot{\Phi}}{{\frac{U}{\nu_0} }} \cdot (\Phi + w \dot{\Phi}) $$

$$ \ddot{\Phi} \approx - k (\Phi + w \dot{\Phi}), \quad k = R( 1 -\frac{\nu_0}{U}) $$

	\item  $  \mathbb{I}_{q_0} = 0,  \mathbb{I}_{q_1} = 1 $
	
		$$ h_0 = \frac{\dot{\Phi} + \frac{U}{\nu_1} - 1}{\frac{U}{\nu_1}} \stackrel{\dot \Phi \to 0}{\to} \frac{U - \nu_1}{U} ,\quad 1 - h_0 = \frac{ 1 - \dot{\Phi}}{{\frac{U}{\nu_1} }} . $$

$$ \frac{\ddot{\Phi}}{\frac{U}{\nu_1} } = -R \frac{\dot{\Phi} + \frac{U}{\nu_1} - 1}{\frac{U}{\nu_1}} \cdot \frac{ 1 - \dot{\Phi}}{{\frac{U}{\nu_1} }} \cdot (\Phi + w \dot{\Phi}) $$

$$ \ddot{\Phi} \approx - k (\Phi + w \dot{\Phi}), \quad k = R( 1 -\frac{\nu_1}{U}) $$

	\item  $  \mathbb{I}_{q_0} = 0,  \mathbb{I}_{q_1} = 0 $ 
	
	$$ \frac{d}{d\theta} \ln \frac{h_0}{1-h_0} = \frac{\dot{h_0}}{h_0 (1-h_0)} = R(\tau_1 - \tau_0)$$
	
	$$ h_0(\theta) = \sigma \left( \ln \frac{h_0(\theta_0)}{1 - h_0(\theta_0)} + R(\tau_1 - \tau_0)(\theta - \theta_0) \right) \stackrel{\theta \to  \infty}{\to} 1, \quad \sigma(x) = \frac{1}{1 + e^{-x}}$$
 
 \end{enumerate}

For equation $\ddot{\Phi} + k (\Phi + w \dot{\Phi}) = 0$ we can estimate the solution decay rate:
$$ w \leq \frac{2}{\sqrt{k}}: \quad t_0 - t_1, h_0 - h^* \propto e^{-\frac{kw}{2} \theta}$$ 
$$w > \frac{2}{\sqrt{k}}: \quad t_0 - t_1, h_0 - h^* \propto e^{-\frac{kw - \sqrt{(kw)^2 - 4k}}{2}\theta}$$

\subsection*{Case switching}

We have invariants $\Phi$, and $h_0$. Below we study the derivative switch $ \dot{\Phi} \to \dot{\Phi'} $. 

\begin{itemize}

	\item $1 \to 2$. Necessary condition: $h_0 > 1 - \frac{\nu_1}{U}$.
$$ \frac{\dot{\Phi} + \frac{U}{\nu_1}}{\frac{U}{\nu_0} + \frac{U}{\nu_1}} = \frac{\dot{\Phi'} + 1}{\frac{U}{\nu_0}}$$		
$$ \dot{\Phi'} = \frac{\dot{\Phi} - \frac{ \nu_0 + \nu_1 - U }{\nu_1} }{\frac{\nu_0 + \nu_1}{\nu_1}} $$
We are either close to equilibrium, or decrease $|\dot{\Phi}|$:
$$ - \frac{\nu_0 + \nu_1 - U}{\nu_0} < \dot{\Phi} < \frac{\nu_0 + \nu_1 - U}{\nu_0 + 2\nu_1} \quad \Rightarrow \quad  | \dot{\Phi'}| < \frac{\nu_0 + \nu_1 - U}{\nu_0} $$
$$ \dot{\Phi} \geq \frac{\nu_0 + \nu_1 - U}{\nu_0 + 2\nu_1}  \quad \Rightarrow \quad |\dot{\Phi'}| \leq |\dot{\Phi}| $$

	\item $1 \to 3$. Necessary condition: $h_0 < \frac{\nu_0}{U}$.
$$  \frac{\dot{\Phi} + \frac{U}{\nu_1}}{\frac{U}{\nu_0} + \frac{U}{\nu_1}} = \frac{\dot{\Phi'} + \frac{U}{\nu_1} - 1}{\frac{U}{\nu_1}} $$
$$ \dot{\Phi'} = \frac{ \dot{\Phi} + \frac{\nu_0 + \nu_1 - U}{\nu_0} }{ \frac{\nu_0 + \nu_1}{\nu_0} } $$
 $|\dot{\Phi}|$ decreases:
$$ \dot{\Phi} > \frac{\nu_0 + \nu_1 - U}{\nu_1} \quad \Rightarrow \quad |\dot{\Phi'}| < | \dot{\Phi} | $$

	\item $2 \to 1$. Necessary condition: $h_0 = 1 - \frac{\nu_1}{U}$.
$$     \frac{\dot{\Phi} + 1}{\frac{U}{\nu_0}} = \frac{\dot{\Phi'} + \frac{U}{\nu_1}}{\frac{U}{\nu_0} + \frac{U}{\nu_1}} = 1 - \frac{\nu_1}{U} $$
 $$ \dot{\Phi}= \dot{\Phi'} = - \frac{\nu_0 + \nu_1 - U}{\nu_0}$$

	\item $3 \to 1$. Necessary condition: $h_0 = \frac{\nu_0}{U}$.
$$ \frac{ \dot{\Phi} + \frac{U}{\nu_1} - 1}{\frac{U}{\nu_1}} = \frac{\dot{\Phi'} + \frac{U}{\nu_1}}{\frac{U}{\nu_0} + \frac{U}{\nu_1}} = \frac{\nu_0}{U} $$
$$ \dot{\Phi}= \dot{\Phi'} = \frac{\nu_0 + \nu_1 - U}{\nu_1}$$


	\item $ 2/3 \to 4 \to 2$. Necessary condition: $h_0 = \frac{\nu_0}{U}$.
	\\
	Since there are no queues during case 4, we have $\Phi = \Phi' = \tau_0 -\tau_1$. Also, $\dot{\Phi'} = 0$, so we come closer to the equillibrium

	

\end{itemize}

\subsubsection*{Lyapunov Theory}
Our differential equation has form $ \ddot{\Phi} = f(\Phi, \dot{\Phi})$, where $f$ is a polynomial. We view it as autnomous system with Lipshitz RHS
$$  \frac{d}{d\theta} \begin{bmatrix} \Phi \\ \dot{\Phi} \end{bmatrix} = \begin{bmatrix} \dot{\Phi} \\ f(\Phi, \dot{\Phi}) \end{bmatrix} $$
In this case Lyapunov Theory is applicable
\begin{theorem}(Global asymptotic stability) 
Let $V: \mathbb{R}^2 \to \mathbb{R}$ be a continuously differentiable function, s.t. :
$$V(0,0) = 0 \text{ and } \forall (\Phi, \dot{\Phi}) \neq (0, 0): ~V(\Phi, \dot{\Phi}) > 0  , $$
$$ \sqrt{\Phi^2 + \dot{\Phi}^2 } \to \infty \quad \Rightarrow \quad V(\Phi, \dot{\Phi}) \to \infty, $$
$$ \forall (\Phi, \dot{\Phi}) \neq (0, 0):  ~\dot{V}(\Phi, \dot{\Phi}) = \frac{\partial V}{\partial \Phi} \dot{\Phi} + \frac{\partial V}{\partial \dot{\Phi}} f(\Phi, \dot{\Phi}) < 0 $$
Then $(\Phi, \dot{\Phi}) = (0, 0)$ is globally asymptotically stable.
\end{theorem}

\begin{theorem}(Local asymptotic stability)
Let $A = \begin{bmatrix} 0 & 1 \\ \frac{\partial f}{\partial \Phi}(0,0) & \frac{\partial f}{\partial \dot{\Phi}}(0,0) \end{bmatrix}$. If we have $\mathrm{Re} (\lambda_i(A)) < 0$ for both eigenvalues, then $(\Phi, \dot{\Phi}) = (0, 0)$ is locally asymptotically stable.

\end{theorem}

\subsubsection*{Local stability}
Linearized equation $\ddot{\Phi} = \frac{\partial f}{\partial \Phi}(0,0) \cdot \Phi + \frac{\partial f}{\partial \dot{\Phi}}(0,0) \cdot \dot{\Phi} = -k\Phi - kw\dot{\Phi}$.

$$ \mathrm{det} \left( \begin{bmatrix} -\lambda & 1 \\ -k & -kw - \lambda \end{bmatrix} \right) = \lambda^2 + kw \lambda + k; \quad D = k^2w^2 - 4k. $$
Since $k, w > 0$, both eiganvalues have negative real parts for any $D$.
\\
Hence, we always have local asymptotic stability.

\subsubsection*{Sufficient conditions for global stability}
In case $i \in \{ 1, 2, 3 \}$ we can write the equation as
$$ \ddot{\Phi} = - C_i h_0(1-h_0)(\Phi + w \dot{\Phi}).$$ 
Denote 
$$ C := \min_{i \in \{ 1, 2, 3 \}} C_i = \min \left\{ R \left( \frac{U}{\nu_0} + \frac{U}{\nu_1} \right) , R \frac{U}{\nu_0} , R \frac{U}{\nu_1} \right\} = \frac{R U}{\max \{ \nu_0, \nu_1 \}}.$$
Further, assume that
 $$ \forall \theta \geq 0: \quad h_0(\theta) \in [a, b] \text{ with } a > 0, b < 1$$
  and denote  $m := \min_{x \in [a,b]} x(1-x) > 0 $.
\\
Consider $V(\Phi, \dot{\Phi}) = \Phi^2 + (\Phi + w \dot{\Phi}) ^2 >0 $.
$$ \dot{V} = \frac{\partial V}{\partial \Phi} \dot{\Phi} + \frac{\partial V}{\partial \dot{\Phi}} \cdot \left( -C_i  h_0(1-h_0)(\Phi + w \dot{\Phi}) \right)  = $$
$$ = \left( 4\Phi\dot{\Phi} + 2w\dot{\Phi}^2 \right) - 2w C_i h_0(1-h_0)(\Phi + w \dot{\Phi})^2 \leq \left(  4\Phi\dot{\Phi} + 2w\dot{\Phi}^2 \right) - 2wCm (\Phi + w \dot{\Phi})^2 = $$
$$ = 2w \left( \frac{1}{w^2} - Cm \right)  (\Phi + w \dot{\Phi})^2 - \frac{2}{w} \Phi^2  .$$
\\
We can guarantee $\dot{V} < 0$ if $w \geq \frac{1}{\sqrt{Cm}}$.
\\
For $R = 0.1, U = 4.5, [a,b] = [0.01, 0.99]$ we need $w \geq \frac{1}{\sqrt{ \frac{0.1 \cdot 4.5}{3} \cdot 0.01 \cdot .99}} \approx 25.95 $.
\\
Suppose we have $V = \Phi^2 + (\Phi + w\dot{\Phi})^2 \leq B^2$. Then it follows that $ |\Phi| \leq B $, $ | \dot{\Phi} | \leq \frac{\sqrt{2}B}{w} $. 
\\
If we can reach $V = B^2$ s.t. $\frac{\sqrt{2}B}{w} = \frac{\nu_0 + \nu_1 - U}{\nu_0} $ with case switching phase, it guarantees that  we stop case switching and converge to zero.

\newpage

\subsubsection*{Max demand ($U = \nu_0 + \nu_1$)}


Case 4 not possible; Case 1-3 all converge to $h^* := \frac{\nu_0}{U}$.
\\
During the dynamic, queues may form
\\
See Figure \ref{fig:fluctuations_proj}. Figures \ref{fig:amplitudes_proj} and \ref{fig:final_tt_proj} show inflow amplitude decays and final travel times for different projection windows.

\begin{figure}
	\includegraphics[width=0.9\textwidth]{img/replicator_proj_tt.eps}
	\caption{ $ U = 5, R=0.1, \Delta \theta = 0.01$}
	\label{fig:fluctuations_proj}

\end{figure}
	
\begin{figure}
	\includegraphics[width=0.9\textwidth]{img/amplitudes_proj_tt.eps}
	\caption{ Inflow amplitudes for path 0 }
	\label{fig:amplitudes_proj}

\end{figure}

\begin{figure}
	\includegraphics[width=0.9\textwidth]{img/final_tt_proj.eps}
	\caption{ Final travel times }
	\label{fig:final_tt_proj}

\end{figure}

%\begin{figure}
%	\includegraphics[width=0.9\textwidth]{img/replicator_grad_tt.eps}
%	\caption{ Travel time gradient as fitness }
%	\label{fig:replicator_grad_tt}
%
%\end{figure}

\newpage
\subsubsection*{Medium Demand ($ \nu_0 < U < \nu_0 + \nu_1$)}

Different cases have different equilibria:
$$ \frac{\nu_0}{U} > \frac{\nu_0}{\nu_0 + \nu_1} > \frac{U - \nu_1}{U}$$

Figure \ref{fig:case_switching} shows how cases switch until amplitude drops enough and we end up in case $q_0 > 0, q_1 = 0$.

Figure \ref{fig:replicator_medium_demand} shows dynamics for the faster edge 0 with different projection windows. 
Both fitnesses eventually stabilize to values $\phi = -\tau_1$ (negative cost of slower edge).
%It also appears that the queue doesn't form on edge 1, so it has constant fitness $\phi_1(\theta) \equiv - \tau_1 $.

\begin{figure}
	\includegraphics[width=0.9\textwidth]{img/case_switching.pdf}
	\caption{ Case switching }
	\label{fig:case_switching}
\end{figure}


\begin{figure}
	\includegraphics[width=0.9\textwidth]{img/replicator_medium_demand.eps}
	\caption{ Medium demand. $U = 4.5; \Delta\theta = 0.01; R = 0.1$ }
	\label{fig:replicator_medium_demand}

\end{figure}

Now assume that edge 0 operates on full capacity and  edge 1 always operates below capacity, i.e.

$$\dot{t_0}(\theta) = \frac{U\cdot h_0(\theta) - \nu_0}{\nu_0}, \quad
 \dot{t_1}(\theta) \equiv 0 .$$

%This  allows to write the replication equation
%$$ \dot{h}_0 = R \cdot h_0 \cdot (\phi_0 - h_0\phi_0 - (1-h_0)\phi_1) = -R \cdot h_0 \cdot ( 1- h_0 ) \cdot \left( \tau_0 + \frac{1}{\nu_0} (q_0 + w \cdot \frac{\partial q_0}{\partial \theta}) - \tau_1 \right) $$
%in the form
%$$ \ddot{\Phi} = - R \cdot (\Phi + w \dot{\Phi}) \cdot  (1+ \dot{\Phi}) \cdot (1 -  h^* (1+ \dot{\Phi})),$$
% where the following notation is used: 
% $$h^* := \frac{\nu_0}{U}, \quad \Phi(\theta) := t_0(\theta) - t_1(\theta) = \int_0^{\theta} \frac{h_0(z) - h^*}{h^*} dz + \tau_0  - \tau_1 .$$
%  We have $ h_0(\theta) = h^* (1 + \dot{\Phi}(\theta))$ and the assumptions can be written as 
Sufficient conditions of the solution to fulfill the assumptions:
 $$\Phi(\theta) - \Phi(0) \geq 0; \quad \dot{\Phi}(\theta) \geq  - \frac{ \nu_0 + \nu_1 - U}{\nu_0} .$$

%If we further assume that $\dot{\Phi}$ is small (i.e. $h_0$ is close to $h^*$), we can make a simplification and analyze the linear equation
%$$ \ddot{F} = - R \cdot(F + w \dot{F}) \cdot (1-h^*) \quad \Leftrightarrow \quad \ddot{F} + kw\dot{F} + kF = 0 , \quad k = R(1-h^*).$$
%
%This yields a theoretical estimate of decay rate:
%$$ w \leq \frac{2}{\sqrt{k}}: \quad h_0 - h^* \propto e^{-\frac{kw}{2} \theta}$$ 
%$$w > \frac{2}{\sqrt{k}}: \quad h_0 - h^* \propto e^{-\frac{kw - \sqrt{(kw)^2 - 4k}}{2}\theta}$$

Figure \ref{fig:amplitudes_decay} shows that that theoretical decay estimate is good.

\begin{figure}
	\includegraphics[scale=0.5]{img/amplitudes_decay.eps}
	\caption{Amplitudes decay }
	\label{fig:amplitudes_decay}

\end{figure}	

Figure \ref{fig:de_comparison} shows the difference between theoretical and observed dynamics. Used parameters: $ U = 4.5; \Delta\theta = 0.01;  h_0(0) = 0.5;  R = 0.1; w = 1.0 $

\begin{figure}
	\includegraphics[scale=0.75]{img/de_comparison.eps}
	\caption{Solution of DEs compared to the experiment; gray dashed lines show illustrate fulfillment of assumptions }
	\label{fig:de_comparison}

\end{figure}	

Figures \ref{fig:replicator_inits_w_1} and \ref{fig:replicator_inits_w_opt} show dynamics for edge 0 with parameters $U = 4.5; \Delta\theta = 0.01; R = 0.1$ for different initial share with $ w = 1.0 $ and $w = \frac{2}{\sqrt{k}} = 8.49$

\begin{figure}
	\includegraphics[scale=0.5]{img/replicator_inits_w_1.eps}
	\caption{ $ w = 1.0 $ }
	\label{fig:replicator_inits_w_1}

\end{figure}	

\begin{figure}
	\includegraphics[scale=0.5]{img/replicator_inits_w_opt.eps}
	\caption{ $w = \frac{2}{\sqrt{k}} = 8.49$ }
	\label{fig:replicator_inits_w_opt}

\end{figure}	

%\subsection*{Sufficient conditions for convergence}
%
%Suppose we are in case 2 of medium demand setting and assume inflow rate always stays in the neighbourhood of $h^* = \frac{\nu_0}{U}$:
%$$ |h_0(\theta) - h^* | \leq | \frac{\nu_0}{U} - (1 - \frac{\nu_1}{U}) |= \frac{\nu_0 + \nu_1 - U}{U} .$$
%This guarantees no cases switching, as $U (1 - h_0(\theta)) \leq \nu_1$.   
%\\
%Denote $ m := \min_{\theta} h_0(\theta)(1 - h_0(\theta)) > 0 $
%\\
%Consider $V(\Phi, \dot{\Phi}) = \Phi^2 + (\Phi + w \dot{\Phi}) ^2 >0 $.
%$$ \dot{V} = \frac{\partial V}{\partial \Phi} \dot{\Phi} + \frac{\partial V}{\partial \dot{\Phi}} \cdot \left( -\frac{R}{h^*} h_0(1-h_0)(\Phi + w \dot{\Phi}) \right)  = $$
%$$ = \left( 4\Phi\dot{\Phi} + 2w\dot{\Phi}^2 \right) - 2w \frac{R}{h^*} h_0(1-h_0)(\Phi + w \dot{\Phi})^2 \leq \left(  4\Phi\dot{\Phi} + 2w\dot{\Phi}^2 \right) - 2w\frac{Rm}{h^*} (\Phi + w \dot{\Phi})^2 = $$
%$$ = 2w \left( \frac{1}{w^2} - \frac{Rm}{h^*} \right)  (\Phi + w \dot{\Phi})^2 - \frac{2}{w} \Phi^2  .$$
%\\
%We can guarantee $\dot{V} < 0$ for $w \geq \sqrt{\frac{h^*}{Rm}}$. With used parameters that is:
%$$w \geq \sqrt{ \frac{ 2/4.5 }{ 0.1 \cdot 3/4.5 \cdot (1-3/4.5)} } \approx 4.47 .$$


\newpage
\subsection*{Unstable dynamics}

Figures \ref{fig:fluctuations_avg}, \ref{fig:fluctuations_last} and \ref{fig:fluctuations_pred} show how using bad fitness leads to divergence.

\begin{center}
	\begin{figure}
	\includegraphics[scale=0.5]{img/replicator_avg_tt.eps}
	\caption{Fluctuations, average travel time }
	\label{fig:fluctuations_avg}

	\end{figure}
	
\end{center}

\begin{center}
	\begin{figure}
	\includegraphics[scale=0.5]{img/replicator_last_tt.eps}
	\caption{Fluctuations, last travel time }
	\label{fig:fluctuations_last}

	\end{figure}
	
\end{center}

\begin{center}
	\begin{figure}
	\includegraphics[scale=0.5]{img/replicator_pred_tt.eps}
	\caption{Fluctuations, predicted travel time }
	\label{fig:fluctuations_pred}

	\end{figure}
	
\end{center}

\subsubsection*{Proof ?}

Necessary condition for stability: $ \forall P: ~ \phi_P(\theta, h) = \sum_{P'} h_{P'}(\theta) \phi_{P'}(\theta, h) $. \\
In cases of average travel time and last travel, influence of inflows on fitnesses is delayed for at least $\tau_0$. \\ 

Sufficient condition for stability for non-aggregated travel times: queues have to not change for the period of delay. This guarantees that fitnesses don't change once equality is reached.
\\

Even when we use undelayed travel times, inflows tend to get in antiphase with fitnesses.
In this example, we need inflows to equalize with edge capacities at the moment when both path have same costs.


\end{document}